added indexes.

LeanC/Arrays.lean
@@ -1,4 +1,7 @@
 import LeanC.Types
+import LeanC.TypeClasses
+import LeanC.Values
+
 /-!
 # Array Types for lean_c
 
@@ -7,26 +10,34 @@ This module defines core RAM related types:
 CMemoryBlock -- represents pointer to void, but with associated
 allocated size to guarantee within bounds operations.
 
-CArray -- MemoryBlock with Associated Type
+In general we need a proof system that the block of memory is allocated and contains specific number of items.
 
-CSlice -- a subarray (Rust inspired name)
+This splits into 3 cases: stack allocation, RAM allocation and within code allocation (asm data blocks).
 
-In general we need a proof system that the block of memory is allocated.
-This splits into 2 cases: stack allocation and RAM allocation.
-Stack allocations are complicated, since we need to know the size of the stack and have
-a proof that current stack allocation does not break stack allocation. Since the size of the stack
-can sometimes be defined in the compiler options, that requires the interaction with compliter.
-There are also static allocations that are allocated as a part of program. There is guarantee that
-if program is loaded this part of memory is allocated.
+- Stack allocations are complicated, since we need to know the size of the stack and have
+  a proof that current allocation does not exeed stack size. Since the size of the stack
+  can sometimes be defined in the compiler options, that requires the interaction with compliter.
+  We will not use this part now untill we can interoperate with toolchain.
 
-For array reasoning we also need to know the size of allocated block
-in bytes? and in type units. This can be done in 2 ways.
+- There are also global static allocations that are allocated as a part of a program (asm data block).
+  There is guarantee that if program is loaded this part of memory is allocated.
+  We would assume that global static arrays are allocated in data segment.
+  Otherwise, there is no good way to define even "Hello world!" string.
+
+- Dynamically allocaed arrays should have a dedicated pointer variable. It can have 2 states:
+  1. Allocated - with the proof it is allocated
+  2. NotAllocated - not yet initialized or allocation failed.
+
+
+For array reasoning we also need to know the size of allocated block in bytes? and in type units.
+ This can be done in 2 ways.
 
 1. the allocation size is known during compilation time and does not change (like incase of static allocations).
 2. the allocation size is dynamically changing, like when arrays are growing and one have to
    reallocate memory.
 
 Fixed allocations can have allocation size as Nat parameter.
+
 Dynamic allocations should have a variable of integer type that will track the allocation size
 For this we need to define a variable reference type. The difficulty is that the variable can be defined
 very deep inside the function tree, and inside the structures within these functions, and then
@@ -38,6 +49,10 @@ that have the same size, so we need to keep only one size value and reallocate a
 The pointer of the array and size variables can be defined in the allocated memories (say an array
 referencing another arrays). So we need to be sure that at the time of the access to the array variables these pointers are stil allocated.
 
+So ingeneral, CArray class should have an information about pointer, allocation state and allocated size.
+It should support a proof that when element of an array is accessed it is in allocated array, and
+the element is entierly within allocated region.
+
 We need to define CMemoryAllocation operation that have 2 branches: succesfull allocation and failure.
 Two branches have two different types of variables
 
@@ -45,10 +60,59 @@ we can have either smart or private constructors in lean to prevent unauthorized
 
 Anfortunately at this level of description we can have only `sorry` proof for memory allocations.
 The real proof would require a system allocation core to be implemented within this system.
+
+
 -/
 
 namespace LeanC
 universe u
+
+/-- we need to denote an index of an array.
+  index can be a Natural value, or it can be a variable with non-negative value.
+  We cannot access the region before the allocated region.
+ -/
+class CIndex ( α : Type ) where
+  isIndex : Prop
+
+/-- CArray defines a set of propositions to ensure arrays is well behaving -/
+class CArray (α:Type) where
+  /-- when accessing, reallocating and freeing array we need to be sure it is allocated.
+    when allocating array we need to be sure it is not yet allocated, otherwise we get a memory leak.
+  -/
+  isAllocated : Prop
+  /-- for free and reallocation operation we need to be sure the array is still allocated
+    and it was dynamically allocated -/
+  isDynamicallyAllocated : Prop
+  /-- for accessing elements of an array we need to be sure the array is allocated and
+    the indexed element is within allocated region. -/
+  within_bounds (α : Type ) [CIndex α] : Prop
+
+/-- an implementation of constant index as a natural number -/
+inductive CConstIndex (n:Nat) where
+| mk
+instance {n:Nat} : CIndex (CConstIndex n) where
+  isIndex := True
+
+/-- An implementation of index variable, conceptually this can be stored in the
+  CVarScope and behave as any other C variable, but with the rules assigned to it.
+  α is the underlying type of index holding variable. It should be of integer type,
+  but we do not require it to be strictly positive number, since for example we an have a situation
+  where negative number means no value. Therefore, we need a proof that the index is nonegative.
+
+  This will support the scenario when somwone would have an integer variable, but in certain situation
+  can make an index out of integer, for example by checking the the value is non-negative, like
+  if(i>=0) b= a[i];
+
+  uints have the proof by construction that they are nonegative.
+-/
+inductive CVarIndex (α:Type) [IsIntegerType α] [IsIntegerNonnegative α]
+  (non_negative: IsIntegerNonnegative.isNonnegative α ) where
+| mk
+
+example := CVarIndex CUInt64Type (by simp [uint_nonnegative])
+
+------  CONTINUE HERE -------
+
 
 inductive CStaticMemoryBlock (n:Nat) where
 | private mk
