LeanC/Values.lean
@@ -4,7 +4,26 @@ Literal AST and serializers for lean_c - stub.
 -/
 
 
+universe u
+
 namespace LeanC
+
+class IsIntegerNonnegative (α : Type u) [IsIntegerType α] where
+ isNonnegative : Prop
+
+instance {sz : CIntSize} : IsIntegerNonnegative (CIntType sz false) where
+ isNonnegative := True
+
+example := IsIntegerNonnegative.isNonnegative (CIntType CIntSize.I8 false)
+
+theorem uint_nonnegative {sz : CIntSize} :
+  IsIntegerNonnegative.isNonnegative (CIntType sz false) := by
+  simp [IsIntegerNonnegative.isNonnegative]
+
+-- example :=
+--   let t := (CIntType CIntSize.I8 false )
+--   let ( p : IsIntegerNonnegative.isNonnegative t)
+
 
 /-- TypedValue is a value of type β that can be casted (stored) in var of type α -/
 inductive TypedValue (α : Type) [IsCType α] (β :Type) ( v : β) ( can_cast : β -> α -> Prop )
